feat: lift the restriction in `congr` theorems that all function arguments on the lhs must be free variables
see #988

tests/lean/run/988.lean
@@ -33,3 +33,23 @@ example (as : Array (Nat → Nat)) (h : 0 + x < as.size) :
   rfl
 
 example [Decidable p] : decide (p ∧ True) = decide p := by simp -- should work
+
+def Pi.single [DecidableEq ι] {f : ι → Type u} [∀ i, Inhabited (f i)] (i : ι) (x : f i) : ∀ i, f i :=
+  fun j => if h : j = i then h ▸ x else default
+
+structure Set (α : Type u) where of :: mem : α → Prop
+
+instance : CoeSort (Set α) (Type u) where coe s := Subtype s.mem
+
+@[congr]
+theorem dep_congr [DecidableEq ι] {p : ι → Set α} [∀ i, Inhabited (p i)] :
+    ∀ {i j} (h : i = j) (x : p i) (y : α) (hx : x = y), Pi.single (f := (p ·)) i x = Pi.single (f := (p ·)) j ⟨y, hx ▸ h ▸ x.2⟩
+  | _, _, rfl, _, _, rfl => rfl
+
+theorem aux {p : Nat → Set Nat} {i j y : Nat} (x : p j) (h₁ : x = y) (h₂ : i = j) : Set.mem (p i) y := by
+  have := x.2
+  subst h₁ h₂
+  assumption
+
+example {p : Nat → Set Nat} [∀ i, Inhabited (p i)] (i : Nat) (x : p (0 + i)) (y : Nat) : Pi.single (f := (p ·)) (0 + i) x = Pi.single (f := (p ·)) i ⟨x, aux x rfl (Nat.zero_add i).symm ⟩ := by
+  simp
